AbsDen/IGDTT.lean
@@ -6,32 +6,48 @@ namespace IGDTT
 open Lean Lean.Parser
 
 universe u
+
+def Laterrr (α : Type u) : Type u := Unit → α
+def nexttt {α : Type u} (a : Unit → α) : Laterrr α := a
+def appp {α β : Type u} (f : Laterrr (α → β)) (a : Laterrr α) : Laterrr β :=
+  fun _ => f () (a ())
+unsafe def gfixxx {α : Type u} (f : Laterrr α → α) : α := f (nexttt (fun () => gfixxx f))
+
+-- Generalise from Type u to Sort u:
+@[extern "Laterrr"]
 axiom Later : Sort u → Sort u
-axiom next {α : Sort u} : α → Later α
-axiom ap {α β : Sort u} : Later (α → β) → Later α → Later β
+@[extern "nexttt"]
+axiom next {α : Sort u} (a : PUnit → α) : Later α
+@[extern "appp"]
+axiom ap {α β : Sort u} (f : Later (α → β)) (a : Later α) : Later β
+@[extern "gfixxx"]
+axiom gfix {α : Sort u} (f : Later α → α) : α
+axiom gfix.unfold {α : Sort u} (f : Later α -> α) : gfix f = f (next (fun () => gfix f))
+
 notation "▹ " α:100 => Later α
 
-noncomputable instance : Applicative Later where
-  pure := next
+instance : Applicative Later where
+  pure a := next (fun () => a)
   seq f a := ap f (a ())
-
-axiom Later.eq {α : Sort u} (a b : α) : ▹ (a = b) ↔ next a = next b
-axiom ap.compute {α β : Sort u} (f : α → β) (a : α) : ap (next f) (next a) = next (f a)
-axiom ap.id {α : Sort u} (a : ▹ α) : ap (next id) a = a
-
-axiom gfix {α : Sort u} : (▹ α → α) → ▹ α
-axiom gfix.unfold {α : Sort u} (f : ▹ α -> α) : gfix f = next (f (gfix f))
-
-axiom DLater : ▹ (Sort u) → Sort u
-axiom DLater.next_eq {α : Sort u} : ▹ α = DLater (next α)
-notation "▸ " α:100 => DLater α
 
 declare_syntax_cat nextElem
 syntax (name := nextElem) ident Term.optType ppSpace Term.leftArrow term : nextElem
 syntax (name := delayedSubst) "next[" nextElem,* "]." term : term
 macro_rules
-  | `(term| next[]. $e) => `(pure $e)
+  | `(term| next[]. $e) => `(next (fun () => $e))
   | `(term| next[ $x:ident ← $e₁ ]. $e₂) => `(pure (fun $x => $e₂) <*> $e₁)
   | `(term| next[ $x:ident : $t ← $e₁ ]. $e₂) => `(pure (fun $x : $t => $e₂) <*> $e₁)
   | `(term| next[ $x:ident ← $e₁, $es,* ]. $e₂) => `((next[ $es,* ]. (fun $x => $e₂)) <*> $e₁)
   | `(term| next[ $x:ident : $t ← $e₁, $es,* ]. $e₂) => `((next[ $es,* ]. (fun $x : $t => $e₂)) <*> $e₁)
+
+axiom Later.eq {α : Sort u} {a b : α} : ▹ (a = b) ↔ (next[].a) = (next[].b)
+axiom ap.compute {α β : Sort u} (f : α → β) (a : α) : ap (next[].f) (next[].a) = next[].(f a)
+axiom ap.id {α : Sort u} (a : ▹ α) : ap (next[].id) a = a
+
+axiom DLater : ▹ (Sort u) → Sort u
+axiom DLater.next_eq {α : Sort u} : ▹ α = DLater (next[].α)
+notation "▸ " α:100 => DLater α
+
+-- protected def Later.recOn {α : Type u} {motive : ▹ α → Type u} : (l : ▹ α) → ▹ ((a : α) → motive (next a)) → motive l :=
+--   cannot have this! Otherwise, it would be possible to recOn (▹ False)
+--   sorry
